sigma.v
@@ -1,15 +1,16 @@
 Require Import Program Arith ZArith Lia.
-
+Theorem th1: forall a b :nat, forall a0 b0: nat, b0 - a0 < b - a -> 0 < b - a.
+Proof.
+  intros.
+  lia.
+  Qed.
+  
  Program Fixpoint solution_1 (f: nat -> Z) (a b: nat) {measure (b - a)}: Z :=
   if Nat.ltb b a then 0
   else if Nat.eqb a b then f a
   else f a + solution_1 f (a + 1) b.
 
   Next Obligation.
-   
-    
-    
-
   
 
 Program Fixpoint solution_2 (f: nat -> nat) (a b : nat) {measure (b-a)} : nat :=
